---
title: 'Lista 6'
author: 'Allan'
date: '02/04/2021'
output: 
    pdf_document: 
        extra_dependencies: ['mathtools']
        latex_engine: pdflatex
---

# Questão 1

$$
p(x)=
\begin{cases}
    \frac{1}{N} &,\;x\in\{1,...,N\}\\
    0 &,\;c.c\\
\end{cases}$$

$$
EX=\sum_x xp(x)=
\sum_{x=1}^N \frac{x}{N}=
\frac{N(N+1)}{2}\frac{1}{N}=
\frac{N+1}{2}
$$

$$
EX^2=\sum_x x^2p(x)=
\sum_{x=1}^N \frac{x^2}{N}=
\frac{N(N+1)(2N+1)}{6}\frac{1}{N}=
\frac{(N+1)(2N+1)}{6}
$$

Então
$$\begin{aligned}
VarX&=
EX^2-(EX)^2=
\frac{(N+1)(2N+1)}{6}-\left(\frac{N+1}{2}\right)^2=\\
&=
\frac{(N+1)(2N+1)}{6}-\left(\frac{N+1}{2}\right)^2=
\frac{2(N+1)(2N+1)-3(N+1)(N+1)}{12}=\\
=&
\frac{(N+1)(2(2N+1)-3(N+1))}{12}=
\frac{(N+1)(4N+2-3N-3)}{12}=
\frac{(N+1)(N-1)}{12}=\\
=&
\frac{N^2-1}{12}
\end{aligned}$$


# Questão 2

## a)

$$\lim_{X\rightarrow \infty} \frac{(X+1)^{-(r+2)}}{X^{-(r+2)}}=...$$

$$\sum_{x=1}^\infty \frac{1}{c}x^{-(r+2)}=1
\Rightarrow c=\sum_{x=1}^\infty x^{-(r+2)}$$

## b)

$$EX^r=
\sum_{x=1}^\infty x^r \frac{x^{-(r+2)}}{\sum_{x=1}^\infty x^{-(r+2)}}=
\sum_{x=1}^\infty \frac{x^{-2}}{\sum_{x=1}^\infty x^{-(r+2)}}=
\sum_{x=1}^\infty \frac{1}{\sum_{x=1}^\infty x^{-(r+2)+2}}=
\sum_{x=1}^\infty \frac{1}{\sum_{x=1}^\infty x^{-r}}=
$$

# Questão 3

$$\begin{aligned}
EX^2=&
\sum_x x.x p_x(x)=
\sum_{x=r}^{\infty}
x.x {x-1 \choose r-1}p^r(1-p)^{x-r}=
\sum_{x=r}^{\infty}
\frac{x.x!}{(x-r)!(r-1)!}p^r(1-p)^{x-r}=\\
=&
\sum_{x=r}^{\infty}
\frac{r}{r}\frac{x.x!}{(x-r)!(r-1)!}p^r(1-p)^{x-r}=
\sum_{x=r}^{\infty}
r\frac{x.x!}{(x-r)!(r)!}p^{r+1-1}(1-p)^{x-r}=\\
=&
\frac{r}{p}
\sum_{x=r}^{\infty}
x{x \choose r}p^{r+1}(1-p)^{x-r}=
\frac{r}{p}\frac{r}{p}
\end{aligned}$$
...

# Questão 4

$$Var(X^2Y)=
E(X^2Y)^2-(E(X^2Y))^2=EX^4EY^2-(EX^2EY)^2=2.1-0=2$$


# Questão 5

## a)

$$E\bar{X}=
E\left(\frac{\sum_{i=1}^n X_i}{n}\right)=
\frac{1}{n}\sum_{i=1}^n E\left(X_i\right)=
\frac{1}{n}\sum_{i=1}^n \mu=\mu$$

## b)

$$Var\bar{X}=
Var\left(\frac{\sum_{i=1}^n X_i}{n}\right)=
\frac{1}{n^2}\sum_{i=1}^n Var\left(X_i\right)=
\frac{1}{n^2}\sum_{i=1}^n \sigma^2=\frac{\sigma^2}{n}$$

## c)

$$\begin{aligned}
E\left[\sum_{i=1}^n (X_i-\bar{X})^2\right]=&
\sum_{i=1}^n E\left[ (X_i-\bar{X})^2\right]=
\sum_{i=1}^n E\left[ X_i^2-2X_i\bar{X}+\bar{X}^2\right]=\\
=&
\sum_{i=1}^n E[X_i^2]-2E[X_i\bar{X}]+E[\bar{X}^2]=\\
=&
\sum_{i=1}^n (\sigma^2+\mu^2)-2E[X_i]E[\bar{X}]+(\frac{\sigma^2}{n}+\mu^2)=\\
=&
\sum_{i=1}^n (\sigma^2+\mu^2)-2\mu^2+(\frac{\sigma^2}{n}+\mu^2)=\\
=&
\sum_{i=1}^n \sigma^2+\frac{\sigma^2}{n}=
\sum_{i=1}^n \sigma^2(1+\frac{1}{n})=\\
=&
\sigma^2(n+1)
\end{aligned}
$$

# Questão 6

## a)

## b)

# Questão 7

$$\begin{aligned}
    \rho(X_1-X_2,X_2+X_3)=&
    \frac{Cov(X_1-X_2,X_2+X_3)}{\sqrt{(\sigma_1^2-\sigma_2^2)(\sigma_2^2+\sigma_3^2)}}=
    \frac{E[(X_1-X_2)(X_2+X_3)]-E[(X_1-X_2)]E[(X_2+X_3)]}{\sqrt{(\sigma_1^2-\sigma_2^2)(\sigma_2^2+\sigma_3^2)}}=\\
    =&
    \frac{E[(X_1X_2+X_1X_3-X_2X_2-X_2X_3)]-E[(X_1-X_2)]E[(X_2+X_3)]}{\sqrt{(\sigma_1^2-\sigma_2^2)(\sigma_2^2+\sigma_3^2)}}=\\
    =&
    \frac{E[X_1X_2]+E[X_1X_3]-E[X_2X_2]-E[X_2X_3]-(E[X_1]-E[X_2])(E[X_2]+E[X_3])}{\sqrt{(\sigma_1^2-\sigma_2^2)(\sigma_2^2+\sigma_3^2)}}=\\
    =&
    \frac{E[X_1X_2]+E[X_1X_3]-E[X_2X_2]-E[X_2X_3]-E[X_1]E[X_2]-E[X_1]E[X_3]+E[X_2]E[X_2]+E[X_2]E[X_3]}{\sqrt{(\sigma_1^2-\sigma_2^2)(\sigma_2^2+\sigma_3^2)}}=
    \\
    =&
    \frac{-E[X_2^2]+E[X_2]^2}{\sqrt{(\sigma_1^2-\sigma_2^2)(\sigma_2^2+\sigma_3^2)}}=
    \frac{-(E[X_2^2]-E[X_2]^2)}{\sqrt{(\sigma_1^2-\sigma_2^2)(\sigma_2^2+\sigma_3^2)}}=\\
    =&
    \frac{-\sigma_2^2}{\sqrt{(\sigma_1^2-\sigma_2^2)(\sigma_2^2+\sigma_3^2)}}
\end{aligned}$$

# Questão 8

$$\rho(X,Y)=\frac{a}{\sqrt{1.2}}=
\frac{1}{2}\Rightarrow a=\frac{\sqrt{2}}{2}=Cov(X,Y)$$

Assim

$$\begin{aligned}
Var(X-2Y)=&
Var(X)+Var(-2Y)-2Cov(X,-2Y)=\\
=&
Var(X)+4Var(Y)+4Cov(X,Y)=\\
=&
1+8+4\frac{\sqrt{2}}{2}=\\
=&
9+2\sqrt{2}
\end{aligned}$$

# Questão 9

# Questão 10

